% !TEX program = xelatex

%This document had would had been used on Ways to Singularity, which is a website that supports MathJax. So some html elements may occur in this document. DELETE THIS when publishing. (If you are not very clear on the grammar I used here, read the academic publication called Time Traveller's Handbook of 1001 Tense Formations by Dr Dan Streetmentioner, which had would had been publish in year 220010 of Gregorian Calendar.)

\documentclass[12pt,a4paper]{article}


%%%%% Page settings  %%%%%
\addtolength{\textheight}{2.0cm}
\addtolength{\voffset}{-2cm}
\addtolength{\hoffset}{-1.0cm}
\addtolength{\textwidth}{2.0cm}

%\allowdisplaybreaks


%%%%%% Math %%%%%%%
\usepackage{amsthm,amsfonts,amssymb,bm}
\usepackage{mathrsfs}
\usepackage[fleqn]{amsmath}
\usepackage{subeqnarray}




%%%%% MISC  %%%%%%

%\usepackage{color}
\usepackage[usenames,dvipsnames]{color}
\usepackage{url}
\usepackage{ulem}
\usepackage{indentfirst}   % Indent first line of a paragraph
%\usepackage{textcomp}

\usepackage{enumerate}


%%%%%%   Here is the configuration for chinese. setmainfont is the default font of the text.
%\usepackage[cm-default]{fontspec}
%\usepackage{xunicode}
%\usepackage{xltxtra}
%\setmainfont{Arial}
%\setsansfont[BoldFont=Arial]{KaiTi_GB2312}
%\setmonofont{NSimSun}


%\XeTeXlinebreaklocale "zh"
%\XeTeXlinebreakskip = 0pt plus 1pt

% Redefine some fonts.
%\newfontfamily\heiti{"黑体"}
%\newfontfamily\fs{"仿宋"}
%\newfontfamily\yahei{"微软雅黑"}


%%%%%%% Figure, Diagram, Caption settings  %%%%%
%\usepackage{tikz}
%\usetikzlibrary{mindmap,trees}

\usepackage{graphicx}
%\usepackage{graphics}
%\usepackage[hang,small,bf]{caption}
%\setlength{\captionmargin}{50pt}


%\graphicspath{{Figures/}



%includeonly{}

\begin{document}
%\title{TITLE}
%\author{{\bf MA} Lei  \\
%@ Interplanetary Immigration Agency \\
%{\small\em \copyright \ Draft date \today}}
%\date{}
%\maketitle


%%%%%% Redefine some math commands and environments. %%%%

\newcommand{\dd}{\mathrm d}

%\newcommand{\HH}{\mathcal H}

%\newcommand{\CN}{{\it Cosmologia Notebook}}

%\newenvironment{eqnset}
%{\begin{equation}\left \bracevert \begin{array}{l}}
%{\end{array} \right. \end{equation}}

%\newenvironment{eqn}
%{\begin{equation}\left \bracevert \begin{array}{l}}
%{\end{array} \right. \end{equation}}


%%%%%%%%%%%%%%%%%%%%%%%%%%%%%%%%%%%%%%%%%%%%%%%%%%%%%%%%
%%%%%%%%%%%%%%    Let's Start Typing     %%%%%%%%%%%%%%%
%%%%%%%%%%%%%%%%%%%%%%%%%%%%%%%%%%%%%%%%%%%%%%%%%%%%%%%%





%%%%%%%%  Tensors and Local Symmetries   %%%%%%%%%%
\section{Tensors and Local Symmetries}

\begin{enumerate}
\item

Transformation from euclidean (x,y) to polar (r,$\theta$) is
\begin{equation*}
	\begin{cases}
	x= r\cos\theta \\
	y= r\sin\theta
	\end{cases}
\end{equation*}

Transformation from polar to euclidean coordinates is
\begin{equation*}
	\begin{cases}
	r= \sqrt{x^2 + y^2} \\
	\cos\theta= x/r \\
	\sin\theta=y/r \\
	\theta = \arccos{\frac{x}{\sqrt{x^2+y^2}}} \qquad \text{for positive y} \\
	\theta = \pi + \arccos{\frac{x}{\sqrt{x^2+y^2}}} \qquad \text{for negative y}
	\end{cases}
\end{equation*}

Partial derivatives

\begin{eqnarray*}
&&\frac{\partial r}{\partial x} = \frac{\partial{\sqrt{x^2 + y^2}}}{\partial x} = \frac{ x }{ \sqrt{x^2 + y^2} } = \frac x r \\
&& \frac{ \partial x }{ \partial r } = \frac{ \partial r\cos\theta }{ \partial r } = \cos\theta = \frac x r
\end{eqnarray*}

\begin{eqnarray*}
&&\frac{ \partial r }{ \partial y } = \frac{\partial \sqrt{x^2 + y^2} }{ \partial y } = \frac{ y }{ \sqrt{x^2 + y^2} } = \frac y r \\
&&\frac{ \partial y }{ \partial r } = \frac{ \partial r\sin\theta }{ \partial r } = \sin\theta = \frac{y}{r}
\end{eqnarray*}

\begin{eqnarray*}
&& \frac{ \partial\theta }{ \partial x } = \frac{ \partial\arccos{\frac{x}{\sqrt{x^2+y^2}} } }{ \partial x } = \frac{-1}{\sqrt{1 - \frac{x^2}{x^2+y^2} }} \frac{y^2}{(x^2+y^2)^{3/2}} = \frac{-y}{x^2+y^2} = -\frac{y}{r^2} \\
&& \frac{\partial x}{\partial \theta} = \frac{\partial r\cos\theta}{\partial \theta} = -r\sin\theta = -y
\end{eqnarray*}
{\color{red}{Page 432 equation 11.23?}}


\begin{eqnarray*}
&& \frac{ \partial \theta }{ \partial y } = \frac{ \partial\arccos{\frac{x}{\sqrt{x^2+y^2}} } }{ \partial y } = \frac{-1}{\sqrt{1 - \frac{x^2}{x^2+y^2} }} \frac{-xy}{(x^2+y^2)^{3/2}} = \frac{x}{x^2+y^2} = \frac{x}{r^2} \\
&& \frac{ \partial y }{ \partial \theta } = \frac{ r\sin\theta }{ \partial \theta } = r\cos\theta = x
\end{eqnarray*}

To summarize

\begin{eqnarray}
\frac{\partial \theta}{\partial x} =-\frac{y}{r^2} &\neq& \frac{\partial x}{\partial\theta} = -y \\
\frac{\partial \theta}{\partial y} = \frac{x}{r^2} &\neq& \frac{\partial y}{\partial\theta} =  x
\end{eqnarray}



%%%%%%%%%%%%% 11.2 %%%%%%%%%%
\item



%%%%%%%  11.3 %%%%%%%
\item

Put 

\begin{equation}
L =  
	\begin{pmatrix}
\gamma & \beta & 0 & 0 \\
\beta & \gamma & 0  & 0 \\
0 & 0 & 1 & 0 \\
0 & 0 & 0 & 1
	\end{pmatrix}
\end{equation}

into $L^T \eta L$.

\begin{eqnarray}
L^T \eta L 
&=& 
\begin{pmatrix}
\gamma & \beta & 0 & 0 \\
\beta & \gamma & 0  & 0 \\
0 & 0 & 1 & 0 \\
0 & 0 & 0 & 1
	\end{pmatrix} 
		\begin{pmatrix}
-1 & 0 & 0 & 0 \\
0 & 1 & 0  & 0 \\
0 & 0 & 1 & 0 \\
0 & 0 & 0 & 1
	\end{pmatrix}
	\begin{pmatrix}
\gamma & \beta & 0 & 0 \\
\beta & \gamma & 0  & 0 \\
0 & 0 & 1 & 0 \\
0 & 0 & 0 & 1
	\end{pmatrix}  \\
&=&
\begin{pmatrix}
-\gamma & \beta & 0 & 0 \\
-\beta & \gamma & 0  & 0 \\
0 & 0 & 1 & 0 \\
0 & 0 & 0 & 1
	\end{pmatrix}
		\begin{pmatrix}
\gamma & \beta & 0 & 0 \\
\beta & \gamma & 0  & 0 \\
0 & 0 & 1 & 0 \\
0 & 0 & 0 & 1
	\end{pmatrix} \\
&=& 
	\begin{pmatrix}
\beta^2-\gamma^2 & 0 & 0 & 0 \\
0 & -\beta^2+\gamma^2 & 0  & 0 \\
0 & 0 & 1 & 0 \\
0 & 0 & 0 & 1
	\end{pmatrix}
\end{eqnarray}

Since $\beta=\sqrt{\gamma^2-1}$,
\begin{equation}
L^T\eta L = 
	\begin{pmatrix}
-1 & 0 & 0 & 0 \\
0 & 1 & 0  & 0 \\
0 & 0 & 1 & 0 \\
0 & 0 & 0 & 1
	\end{pmatrix} = \eta
\end{equation}



%%%%%%%%%%%%%  11.4    %%%%%%%%%%%%%
\item
\begin{equation}
	\eta = L\eta L^T = \Lambda^{-1} \eta(\Lambda^{-1})^T = \Lambda^{-1} \eta(\Lambda^{T})^{-1}
\end{equation}

Inverse both sides
\begin{equation}
	\eta^{-1} = \Lambda^T \eta^{-1} \Lambda
\end{equation}

We already have $\eta^{-1} = \eta$, then
\begin{equation}
	\eta = \Lambda^T \eta \Lambda
\end{equation}



%%%%%%%  11.5  %%%%%%%
\item
To see the same physics means to have the same kinetic energy at center of mass system.

Coordinate transformation leaves scalar unchanged. In this problem, $P_\mu P^\mu$ won't change when we change from one reference frame to another, i.e.,
\begin{equation*}
	-(E_1 + E_2)^2 + m^2 u_2^2c^2 = -(E_1' + E_2')^2 + (m u_1' + m u_2')^2c^2 .
\end{equation*}

We also have
\begin{equation}
	\begin{cases}
	E_2^2=m^2 u_2^2 c^2 + m^2 c^4 \\
	E_1=mc^2 \\
	E_1'=E_2'\\
	u_1'=-u_2'
	\end{cases}
\end{equation}

But the mass of proton is so small compared to the accelerator energy that we can drop $mc^2$ term in our calculation.

Then the energy of the incoming proton in lab frame is
\begin{equation}
	E_2 \approx \frac{2 E_1^2}{mc^2} \approx 10^5 \text{TeV}
\end{equation}




%%%%%%%%%%   11.5   %%%%%%%%%%%%%
\item

Take the divergence of both sides of Maxwell-Ampere law
\begin{eqnarray}
	\nabla \cdot \nabla \times \mathbf B &=& \mu_0 \nabla\cdot\mathbf j + \epsilon_0 \mu_0 \nabla\cdot\dot{\mathbf E} \\
	0 &=& \nabla\cdot \mathbf j + \epsilon_0\nabla\cdot \dot{\mathbf E}
\end{eqnarray}

Divergence of electric field is
\begin{equation}
	\nabla\cdot \mathbf E = \frac \rho {\epsilon_0}
\end{equation}

Thus
\begin{equation}
	0 = \nabla\cdot \mathbf j + \dot{\rho}
\end{equation}


%%%%%%%%%   11.7   %%%%%%%%%%%%
\item

\begin{equation}
	M_{ik} = \frac{1}{2}(M_{ik} + M_{ki}) + \frac{1}{2}(M_{ik} - M_{ki})
\end{equation}
in which the first part is symmetric and the second is antisymmetric.

Exchange $i$ and $k$,
\begin{eqnarray}
	&&\frac12 (M_{ik} + M_{ki})\mathrm dx^i\wedge \mathrm dx^k
	= -\frac12(M_{ki} + M_{ik})\mathrm dx^k\wedge \mathrm dx^i \\
	\rightarrow && (M_{ik} + M_{ki})\mathrm dx^i\wedge \mathrm dx^k = 0
\end{eqnarray}

This shows the symmetric part doesn't contribute to $M_{ik}\mathrm dx^i\mathrm dx^k$.

\begin{eqnarray}
	&&\frac12 (M_{ik} - M_{ki})\mathrm dx^i\wedge \mathrm dx^k
	= \frac12(M_{ki} - M_{ik})\mathrm dx^k\wedge \mathrm dx^i 
	= -\frac12(M_{ki} - M_{ik})\mathrm dx^i\wedge \mathrm dx^k
\end{eqnarray}

Symmetric part contributes to $M_{ik}\mathrm dx^i\mathrm dx^k$.



\begin{eqnarray}
	&&\frac12 (M_{ik} - M_{ki})\mathrm dx^i \mathrm dx^k
	= \frac12(M_{ki} - M_{ik})\mathrm dx^k \mathrm dx^i \\
	\rightarrow && \frac12 (M_{ik} - M_{ki})\mathrm dx^i \mathrm dx^k
	= - \frac12(M_{ik} - M_{ki})\mathrm dx^k \mathrm dx^i \\
	\rightarrow && \frac12 (M_{ik} - M_{ki})\mathrm dx^i \mathrm dx^k =0
\end{eqnarray}


\begin{eqnarray}
	&&\frac12 (M_{ik} + M_{ki})\mathrm dx^i \mathrm dx^k
	= \frac12(M_{ki} + M_{ik})\mathrm dx^k \mathrm dx^i
\end{eqnarray}

Antisymmetric part doesn't contribute to $M_{ik}\mathrm dx^i\mathrm dx^k$.









\end{enumerate}
















\end{document}